src/Verify.v
@@ -30,25 +30,21 @@ Section Verification.
 
   Definition verify_rspec_safety (s : SSA.spec) : bool :=
     let fE := SSA.program_succ_typenv (SSA.sprog s) (SSA.sinputs s) in
-    let es := bb_range_safety_la_simplified s in
+    (* filter is not necessary, it is used to make grat work well *)
+    let es := bb_range_safety_la_simplified_filtered s in
     let '(_, _, _, cnfs) := bb_bexps_cache fE es in
-    (* rev is not necessary, it is used for grat *)
-    let cnfs_rev := map rev cnfs in
-    ext_all_unsat cnfs_rev.
+    ext_all_unsat cnfs.
 
   Lemma verify_rspec_safety_sound (s : SSA.spec) :
     well_formed_ssa_spec s ->
     verify_rspec_safety s ->
     SSA.valid_rspec (SSA.rspec_of_spec s) /\ ssa_spec_safe s.
   Proof.
-    move=> Hwf Hv. apply: (bb_range_safety_la_simplified_sound Hwf).
+    move=> Hwf Hv. apply: (bb_range_safety_la_simplified_filtered_sound Hwf).
     move=> m c g cnfs cnf Hbb Hin. rewrite /verify_rspec_safety in Hv.
     rewrite Hbb in Hv. move: (all_unsat_sound Hv) => Hsat.
-    have Hmem: rev cnf \in [seq rev i | i <- cnfs].
-    { apply: map_f. apply/in_In. exact: Hin. }
-    move: (Hsat (rev cnf) Hmem) => {Hsat} Hsat.
-    move=> Hsat'; apply: Hsat. move/rev_cnf_eqsat : Hsat' => Hsat'.
-    exact: Hsat'.
+    move: (Hsat cnf Hin) => {Hsat} Hsat.
+    move=> Hsat'; apply: Hsat. exact: Hsat'.
   Qed.
 
   Lemma verify_rspec_safety_complete (s : SSA.spec) :
@@ -58,14 +54,11 @@ Section Verification.
   Proof.
     move=> Hwf Hrange Hsafe. rewrite /verify_rspec_safety.
     dcase (bb_bexps_cache (SSA.program_succ_typenv (SSA.sprog s) (SSA.sinputs s))
-                          (bb_range_safety_la_simplified s)) => [[[[m c] g] cnfs] Hbb].
+                          (bb_range_safety_la_simplified_filtered s)) =>
+    [[[[m c] g] cnfs] Hbb].
     apply: all_unsat_complete.
-    move: (bb_range_safety_la_simplified_complete Hwf Hrange Hsafe) => Hv.
-    move=> cs Hin. apply/rev_cnf_eqsat. apply: (Hv _ _ _ _ _ Hbb).
-    clear s Hwf Hrange Hsafe m c g Hbb Hv. elim: cnfs Hin => [| cnf cnfs IH] //= Hin.
-    rewrite in_cons in Hin. case/orP: Hin => Hin.
-    - left. rewrite (eqP Hin). apply: Logic.eq_sym. exact: revK.
-    - right. exact: (IH Hin).
+    move: (bb_range_safety_la_simplified_filtered_complete Hwf Hrange Hsafe) => Hv.
+    move=> cs Hin. apply: (Hv _ _ _ _ _ Hbb). assumption.
   Qed.
 
 
